compiler_test/beepl_test/BeePL_div_zero1.v
@@ -70,4 +70,12 @@ Proof.
   unfold build_bcomposite_env; simpl; reflexivity.
 Qed.
 
-(*Compute (type_check_expr empty_context empty_context f_div_zero.(fn_body)).*)
+(*Definition example1 : BeePL.program := @mkbprogram bcomposites 
+                                                   global_definitions 
+                                                   public_idents 
+                                                   _main 
+                                                   bcomposite_correct
+                                                   ident_to_string.*)
+
+(*Compute (type_check_program example1).*) (* Type checks *)
+
